reshape the proofs to better fit the extension

lean/compiler.lean
@@ -4,6 +4,7 @@ open val bin_op exp instruction
 
 def compile : exp → list instruction
 | (EVal v) := [IPush v]
+| (EVar x) := [ILookup x]
 | (EOp op e₁ e₂) := compile e₂ ++ compile e₁ ++ [IOp op]
 | (EIf c t f) := 
   let t_branch : list instruction := compile t,
@@ -11,3 +12,6 @@ def compile : exp → list instruction
   compile c ++ 
   (IBranch (t_branch.length + 1) :: t_branch) ++ 
   (IJump (f_branch.length) :: f_branch)
+| (ELet x v body) :=
+  -- compiler never leaves "dangling" variables in the environment
+  compile v ++ IOpenScope x :: compile body ++ [ICloseScope]
