lean/semantics.lean
@@ -9,6 +9,46 @@ def eval (n m : ℕ) : ∀ (op : bin_op), val
 | LtOp    := VBool (n < m)
 | EqOp    := VBool (n = m)
 
+def subst (v : val) (x : string) : exp → exp
+|   (EVar y) := if x = y then (EVal v) else (EVar y)
+| l@(ELet y e body) := if x = y then l else ELet y (subst e) (subst body)
+|   (EIf c t e) := EIf (subst c) (subst t) (subst e)
+|   (EOp op e₁ e₂) := EOp op (subst e₁) (subst e₂)
+|   (EVal v) := (EVal v)
+
+def vm_subst' (v : val) (x : string)
+  : list string → list instruction → list instruction
+| nv [] := []
+| nv (ILookup var :: ins) := (if var = x ∧ x ∉ nv then IPush v else ILookup var) :: vm_subst' nv ins
+| nv (IOpenScope var :: ins) := IOpenScope var :: vm_subst' (var :: nv) ins
+| nv (ICloseScope :: ins) := ICloseScope :: vm_subst' nv.tail ins
+| nv (i :: ins) := i :: vm_subst' nv ins
+
+def vm_subst (v : val) (x : string)
+  : list instruction → list instruction := vm_subst' v x []
+
+inductive substitute (v : val) (x : string) : exp → exp → Prop
+| SubVarEq : substitute (EVar x) (EVal v)
+| SubVarNe {y} : y ≠ x → substitute (EVar y) (EVar y)
+| SubVal {v} : substitute (EVal v) (EVal v)
+| SubOp {op e e' f f'} :
+    substitute e e'
+  → substitute f f'
+  → substitute (EOp op e f) (EOp op e' f')
+| SubIf {c c' t t' f f'} :
+    substitute c c'
+  → substitute t t'
+  → substitute f f'
+  → substitute (EIf c t f) (EIf c' t' f')
+| SubLet {x y : string} {e e' body body'} :
+    x ≠ y
+  → substitute e e'
+  → substitute body body'  
+  → substitute (ELet y e body) (ELet y e' body')
+| SubLetShadow {x : string} {e e' body} :
+    substitute e e'
+  → substitute (ELet x e body) (ELet x e' body)
+
 inductive big_step : exp → val → Prop
 | RunVal {v} : big_step (EVal v) v
 | RunOp {op eₙ eₘ n m}
@@ -23,31 +63,84 @@ inductive big_step : exp → val → Prop
     (_ : big_step c (VBool ff))
     (_ : big_step f v)
   : big_step (EIf c t f) v
+| RunLet {e body : exp} {x : string} {v r : val}
+  (_ : big_step e v)
+  (_ : big_step (subst v x body) r)
+  : big_step (ELet x e body) r
 
-infixr ` ⟹ ` : 1 := big_step
+infixr ` ⟹ ` : 30 := big_step
 
 def at_least {α : Type} (n : ℕ) : list α → Prop
 | (l : list α) := l.length ≥ n
 
-inductive vm_big_step : (list instruction × list val) → list val → Prop
-| RunEmpty {stack} : vm_big_step ([], stack) stack
-| RunPush {instrs stack res v}
-    (_ : vm_big_step (instrs, v :: stack) res)
-  : vm_big_step (IPush v :: instrs, stack) res
-| RunOpInstr {instrs stack res op} {n m : ℕ} 
-    (_ : vm_big_step (instrs, eval n m op :: stack) res)
-  : vm_big_step (IOp op :: instrs, VNat n :: VNat m :: stack) res
-| RunTBranch {instrs stack res n}
-    (_ : at_least n instrs)
-    (_ : vm_big_step (instrs, stack) res)
-  : vm_big_step (IBranch n :: instrs, VBool tt :: stack) res
-| RunFBranch {instrs stack res n}
-    (_ : at_least n instrs)
-    (_ : vm_big_step (instrs.drop n, stack) res)
-  : vm_big_step (IBranch n :: instrs, VBool ff :: stack) res
-| RunJump {instrs stack res n}
-    (_ : at_least n instrs)
-    (_ : vm_big_step (instrs.drop n, stack) res)
-  : vm_big_step (IJump n :: instrs, stack) res
+inductive bound : string → val → list (string × val) → Prop
+| bhead {x v env}   : bound x v ((x, v) :: env)
+| btail {x v b env} : bound x v env → bound x v (b :: env)
 
-infix ` ⟹ᵥₘ ` : 1 := vm_big_step
+inductive vm_big_step : 
+  list (string × val) × list instruction × list val → list val → Prop
+| RunEmpty {env stack} : vm_big_step (env, [], stack) stack
+| RunPush {env instrs stack res v}
+    (_ : vm_big_step (env, instrs, v :: stack) res)
+  : vm_big_step (env, IPush v :: instrs, stack) res
+| RunOpInstr {env instrs stack res op} {n m : ℕ} 
+    (_ : vm_big_step (env, instrs, eval n m op :: stack) res)
+  : vm_big_step (env, IOp op :: instrs, VNat n :: VNat m :: stack) res
+| RunTBranch {env instrs stack res n}
+    (_ : vm_big_step (env, instrs, stack) res)
+  : vm_big_step (env, IBranch n :: instrs, VBool tt :: stack) res
+| RunFBranch {env instrs stack res n}
+    (_ : at_least n instrs)
+    (_ : vm_big_step (env, instrs.drop n, stack) res)
+  : vm_big_step (env, IBranch n :: instrs, VBool ff :: stack) res
+| RunJump {env instrs stack res n}
+    (_ : at_least n instrs)
+    (_ : vm_big_step (env, instrs.drop n, stack) res)
+  : vm_big_step (env, IJump n :: instrs, stack) res
+| RunLookup {env x v instrs stack res}
+  (_ : bound x v env)
+  (_ : vm_big_step (env, instrs, v :: stack) res)
+ : vm_big_step (env, ILookup x :: instrs, stack) res
+| RunOpenScope {env x v instrs stack res}
+  (_ : vm_big_step (⟨x, v⟩ :: env, instrs, stack) res)
+  : vm_big_step (env, IOpenScope x :: instrs, v :: stack) res
+| RunCloseScope {env x v instrs stack res}
+  (_ : vm_big_step (env, instrs, stack) res)
+  : vm_big_step (⟨x, v⟩ :: env, ICloseScope :: instrs, stack) res
+
+infix ` ⟹ᵥₘ ` : 25 := vm_big_step
+
+-- big-step semantics including resulting environment
+inductive env_big_step :
+    list (string × val) × list instruction × list val 
+  → list (string × val) × list val → Prop
+| ERunEmpty {env stack} : env_big_step (env, [], stack) (env, stack) 
+| ERunPush {env instrs stack res v}
+    (_ : env_big_step (env, instrs, v :: stack) res)
+  : env_big_step (env, IPush v :: instrs, stack) res
+| ERunOpInstr {env instrs stack res op} {n m : ℕ} 
+    (_ : env_big_step (env, instrs, eval n m op :: stack) res)
+  : env_big_step (env, IOp op :: instrs, VNat n :: VNat m :: stack) res
+| ERunTBranch {env instrs stack res n}
+    (_ : env_big_step (env, instrs, stack) res)
+  : env_big_step (env, IBranch n :: instrs, VBool tt :: stack) res
+| ERunFBranch {env instrs stack res n}
+    (_ : at_least n instrs)
+    (_ : env_big_step (env, instrs.drop n, stack) res)
+  : env_big_step (env, IBranch n :: instrs, VBool ff :: stack) res
+| ERunJump {env instrs stack res n}
+    (_ : at_least n instrs)
+    (_ : env_big_step (env, instrs.drop n, stack) res)
+  : env_big_step (env, IJump n :: instrs, stack) res
+| ERunLookup {env x v instrs stack res}
+  (_ : bound x v env)
+  (_ : env_big_step (env, instrs, v :: stack) res)
+ : env_big_step (env, ILookup x :: instrs, stack) res
+| ERunOpenScope {env x v instrs stack res}
+  (_ : env_big_step (⟨x, v⟩ :: env, instrs, stack) res)
+  : env_big_step (env, IOpenScope x :: instrs, v :: stack) res
+| ERunCloseScope {env x v instrs stack res}
+  (_ : env_big_step (env, instrs, stack) res)
+  : env_big_step (⟨x, v⟩ :: env, ICloseScope :: instrs, stack) res
+
+infix ` ⟹ₙᵥ ` : 25 := env_big_step
