lean/syntax.lean
@@ -15,11 +15,16 @@ inductive exp : Type
 | EVal : val → exp
 | EOp : bin_op → exp → exp → exp
 | EIf : exp → exp → exp → exp
+| EVar : string → exp
+| ELet : string → exp → exp → exp
 
 -- Target language
 
 inductive instruction : Type
-| IPush : val → instruction   -- push val on stack
-| IOp : bin_op → instruction  -- pop two vals, do op, push result
-| IBranch : nat → instruction -- pop a bool, continue if true, else skip n instructions
-| IJump : nat → instruction   -- skip n instructions
+| IPush : val → instruction         -- push val on stack
+| IOp : bin_op → instruction        -- pop two vals, do op, push result
+| IBranch : nat → instruction       -- pop a bool, continue if true, else skip n instructions
+| IJump : nat → instruction         -- skip n instructions
+| ILookup : string → instruction    -- look up the value of a variable and push it
+| IOpenScope : string → instruction -- pop a value and bind it to the name
+| ICloseScope : instruction         -- remove the last variable binding
