lean/proofs/lemmas.lean
@@ -1,0 +1,172 @@
+import ..compiler ..semantics ..syntax ..lovelib
+
+open big_step vm_big_step env_big_step val bin_op exp instruction
+
+-- env_big_step implies vm_big_step
+lemma env_vm_big_step {env env' P S R} :
+    (env, P, S) ⟹ₙᵥ (env', R)
+  → (env, P, S) ⟹ᵥₘ R :=
+begin
+  assume hnv,
+  induction' hnv,
+  case ERunEmpty {
+    apply RunEmpty
+  },
+  case ERunPush {
+    apply RunPush,
+    exact ih
+  },
+  case ERunOpInstr {
+    apply RunOpInstr,
+    exact ih
+  },
+  case ERunTBranch {
+    apply RunTBranch,
+    exact ih
+  },
+  case ERunFBranch {
+    apply RunFBranch,
+    { exact _x },
+    { exact ih }
+  },
+  case ERunJump {
+    apply RunJump,
+    { exact _x },
+    { exact ih }
+  },
+  case ERunLookup {
+    apply RunLookup,
+    { exact _x },
+    { exact ih }
+  },
+  case ERunOpenScope {
+    apply RunOpenScope,
+    exact ih
+  },
+  case ERunCloseScope {
+    apply RunCloseScope,
+    exact ih
+  }
+end
+
+-- generalized intermediate_result lemma
+lemma interm_result_nv 
+  {P₁ P₂ : list instruction} {S S' I : list val} {E₁ E₂ Eᵢ R} :
+    (E₁, P₁, S) ⟹ₙᵥ (Eᵢ, I)
+  → (Eᵢ, P₂, I ++ S') ⟹ₙᵥ (E₂, R)
+  → (E₁, P₁ ++ P₂, S ++ S') ⟹ₙᵥ (E₂, R) :=
+begin
+  assume h1 h2,
+  induction' h1,
+  { exact h2 },
+  { apply ERunPush,
+    rw ←list.cons_append,
+    apply ih h2 },
+  case ERunOpInstr {
+    rw list.cons_append,
+    apply ERunOpInstr,
+    apply ih h2
+  },
+  case ERunTBranch {
+    rw list.cons_append,
+    apply ERunTBranch,
+    apply ih h2
+  },
+  case ERunFBranch {
+    rw list.cons_append,
+    apply ERunFBranch,
+    { rw [at_least, list.length_append], 
+      rw [at_least] at _x,
+      linarith },
+    rw [list.drop_append_of_le_length],
+    apply ih h2,
+    exact _x
+  },
+  case ERunJump {
+    rw list.cons_append,
+    apply ERunJump,
+    { rw [at_least, list.length_append], 
+      rw [at_least] at _x,
+      linarith },
+    rw [list.drop_append_of_le_length],
+    apply ih h2,
+    exact _x
+  },
+  case ERunLookup {
+    apply ERunLookup _x,
+    rw ←list.cons_append,
+    apply ih h2
+  },
+  case ERunOpenScope {
+    rw list.cons_append,
+    apply ERunOpenScope,
+    apply ih h2
+  },
+  case ERunCloseScope {
+    rw list.cons_append,
+    apply ERunCloseScope,
+    apply ih h2
+  }
+end
+
+lemma push_on_stack {P v S R env} : 
+    ((env, IPush v :: P, S) ⟹ₙᵥ R)
+  → ((env, P, [v] ++ S) ⟹ₙᵥ R) :=
+begin
+  intro h,
+  cases' h,
+  exact h
+end
+
+lemma vm_subst_distr {E P₁ P₂ x v S R} : 
+    (E, vm_subst v x P₁ ++ vm_subst v x P₂, S) ⟹ₙᵥ R
+  → (E, vm_subst v x (P₁ ++ P₂), S) ⟹ₙᵥ R :=
+begin
+  assume h,
+  induction' P₁,
+  { exact h },
+  { sorry }
+end
+
+lemma subst_conv {E e x v S R} :
+    (E, compile (subst v x e), S) ⟹ₙᵥ R
+  → (E, vm_subst v x (compile e), S) ⟹ₙᵥ R :=
+begin
+  sorry
+end
+
+lemma extra_bind {E e x v S R} :
+    (E, compile (subst v x e), S) ⟹ₙᵥ R
+  → (E, IOpenScope x :: compile e ++ [ICloseScope], v :: S) ⟹ₙᵥ R := sorry
+
+lemma open_scope_rev {E e x v S R} :
+    (E, IOpenScope x :: compile e ++ [ICloseScope], v :: S) ⟹ₙᵥ R 
+  → ((x, v) :: E, compile e ++ [ICloseScope], S) ⟹ₙᵥ R :=
+begin
+  assume h,
+  cases' h,
+  exact h
+end
+
+lemma open_extra_bind {E E' e x v S S'} :
+    (E, compile (subst v x e), S) ⟹ₙᵥ (E', S')
+  → (⟨x, v⟩ :: E, compile e, v :: S) ⟹ₙᵥ (⟨x, v⟩ :: E', S') :=
+begin
+  assume h,
+  sorry
+end
+
+lemma close_extra_bind {E E' P x v S S'} :
+    (E, P, S) ⟹ₙᵥ (⟨x, v⟩ :: E', S')
+  → (E, P ++ [ICloseScope], S) ⟹ₙᵥ (E', S') :=
+sorry
+
+lemma subst_extra_bind {E e x v S R} :
+    (E, compile (subst v x e), S) ⟹ₙᵥ R
+  → ((x, v) :: E, compile e ++ [ICloseScope], S) ⟹ₙᵥ R := 
+begin
+  assume h,
+  apply open_scope_rev,
+  apply extra_bind,
+  exact h
+end
