lean/proofs/soundness.lean
@@ -1,124 +1,64 @@
-import ..compiler ..semantics ..syntax ..lovelib
+import .lemmas
 
-open big_step vm_big_step val bin_op exp instruction
+open big_step vm_big_step env_big_step val bin_op exp instruction
 
-lemma intermediate_result
-  {P₁ P₂ : list instruction} {S S' I R : list val} :
-    ((P₁, S) ⟹ᵥₘ I) → ((P₂, I ++ S') ⟹ᵥₘ R)
-  → ((P₁ ++ P₂, S ++ S') ⟹ᵥₘ R) :=
-begin
-  assume h1 h2,
-  induction' h1,
-  case RunEmpty { tautology },
-  case RunOpInstr {
-    rw list.cons_append,
-    apply RunOpInstr,
-    apply ih h2
-  },
-  case RunPush {
-    rw list.cons_append,
-    apply RunPush,
-    rw ←list.cons_append,
-    apply ih h2,
-  },
-  case RunTBranch {
-    rw list.cons_append,
-    apply RunTBranch,
-    { rw [at_least, list.length_append], 
-      rw [at_least] at _x,
-      linarith },
-    { apply ih h2 }
-  },
-  case RunFBranch {
-    rw list.cons_append,
-    apply RunFBranch,
-    { rw [at_least, list.length_append], 
-      rw [at_least] at _x,
-      linarith },
-    { rw [list.drop_append_of_le_length _x], 
-      apply ih h2 }
-  },
-  case RunJump {
-    rw list.cons_append,
-    apply RunJump,
-    { rw [at_least, list.length_append], 
-      rw [at_least] at _x,
-      linarith },
-    { rw [list.drop_append_of_le_length _x],
-      apply ih h2 }
-  }
-end
-
-lemma push_on_stack {P v S R} : 
-    ((IPush v :: P, S) ⟹ᵥₘ R)
-  → ((P, [v] ++ S) ⟹ᵥₘ R) :=
-begin
-  intro h,
-  cases' h,
-  exact h
-end
-
-lemma compile_subst
-  {e : exp} {instrs : list instruction} {stack : list val} {v r : val} :
-    ((compile e, []) ⟹ᵥₘ [v])
-  → ((IPush v :: instrs, stack) ⟹ᵥₘ [r])
-  → ((compile e ++ instrs, stack) ⟹ᵥₘ [r]) :=
-assume he hr,
-let h2 := push_on_stack hr in
-intermediate_result he h2
-
-lemma compile_sound (e : exp) (v : val) : 
-    (e ⟹ v) 
-  → ((compile e, []) ⟹ᵥₘ [v]) :=
+lemma compile_sound_nv {e : exp} {v : val} :
+    e ⟹ v
+  → ([], compile e, []) ⟹ₙᵥ ([], [v]) :=
 begin
   assume heval,
   induction' heval,
   case RunVal {
-    rw [compile],
-    apply RunPush,
-    exact RunEmpty 
+    rw compile,
+    apply ERunPush,
+    apply ERunEmpty
   },
   case RunOp {
     rw [compile, list.append_assoc],
-    apply compile_subst ih_heval_1,
-    apply RunPush,
-    apply compile_subst ih_heval,
-    apply RunPush,
-    apply RunOpInstr,
-    apply RunEmpty
+    apply interm_result_nv ih_heval_1,
+    apply interm_result_nv ih_heval,
+    apply ERunOpInstr,
+    apply ERunEmpty
   },
+  case RunLet {
+    rw [compile, list.append_assoc, list.cons_append],
+    apply interm_result_nv ih_heval,
+    apply ERunOpenScope,
+    apply subst_extra_bind,
+    apply ih_heval_1
+  }, 
   case RunIfT {
     rw [compile],
     simp,
-    apply compile_subst ih_heval,
-    apply RunPush,
-    apply RunTBranch,
-    { rw [at_least, 
-          list.length_append, 
-          list.length_cons],
-      linarith },
-    apply compile_subst ih_heval_1,
-    apply RunPush,
-    apply RunJump,
-    { rw [at_least], linarith },
-    rw list.drop_length,
-    apply RunEmpty
+    apply interm_result_nv ih_heval,
+    apply ERunTBranch,
+    apply interm_result_nv ih_heval_1,
+    apply ERunJump,
+    { rw [at_least], simp },
+    { rw [list.drop_length],
+      apply ERunEmpty }
   },
   case RunIfF {
-    rw compile,
+    rw [compile],
     simp,
-    apply compile_subst ih_heval,
-    apply RunPush,
-    apply RunFBranch,
-    { rw [at_least, 
-          list.length_append, 
-          list.length_cons], 
-      linarith },
-    { rw [add_comm, 
+    apply interm_result_nv ih_heval,
+    apply ERunFBranch,
+    { rw [at_least, list.length_append],
+      simp },
+    { rw [nat.add_comm, 
           list.drop_add, 
-          list.drop_left, 
-          list.drop_one, 
+          list.drop_one,
+          list.drop_append_of_le_length,
+          list.drop_length,
+          list.nil_append,
           list.tail],
-      exact ih_heval_1 }
+      exact ih_heval_1,
+      refl }
   }
 end
+
+lemma compile_sound (e : exp) (v : val) : 
+    e ⟹ v
+  → ([], compile e, []) ⟹ᵥₘ [v] :=
+assume hstep, 
+env_vm_big_step (compile_sound_nv hstep)
