lean/proofs/tests.lean
@@ -1,10 +1,11 @@
 import ..syntax ..semantics ..lovelib
 
-open instruction val bin_op vm_big_step
+open instruction exp val bin_op big_step vm_big_step
 
 lemma example1 : 
  vm_big_step
-  ([IPush (VNat 10), 
+  ([], 
+   [IPush (VNat 10), 
     IPush (VNat 20), 
     IOp EqOp, 
     IBranch 1, 
@@ -27,7 +28,7 @@ end
 
 lemma example2 : ¬ ∃ out,
  vm_big_step
-  ([IPush (VNat 10), IPush (VBool false), IOp EqOp], []) out :=
+  ([], [IPush (VNat 10), IPush (VBool false), IOp EqOp], []) out :=
 begin
   assume hexists,
   cases' hexists,
@@ -35,7 +36,8 @@ begin
 end
 
 lemma example3 : 
-  ([IPush (VBool false), 
+  ([],
+   [IPush (VBool false), 
     IBranch 1, 
     IBranch 10,
     IPush (VNat 2),
@@ -63,7 +65,7 @@ end
 
 lemma example4 : 
   ∀ n, n ≠ 0 → 
-  ¬ ∃ out, ([IBranch n], [VBool false]) ⟹ᵥₘ out :=
+  ¬ ∃ out, ([], [IBranch n], [VBool false]) ⟹ᵥₘ out :=
 begin
   assume n hnz hex,
   cases hex with hout hstep,
@@ -72,3 +74,77 @@ begin
   contradiction
 end
 
+lemma unbound_var_no_out₁ : 
+  ¬ ∃ out, EOp PlusOp (EVal (VNat 0)) (EVar "x") ⟹ out := 
+begin
+  assume hex,
+  cases hex with hval hstep,
+  cases hstep,
+  cases hstep__x_1
+end
+
+lemma unbound_var_no_out₂ : 
+  ¬ ∃ out, ELet "y" (EVal (VNat 1)) (EOp PlusOp (EVal (VNat 0)) (EVar "x")) ⟹ out := 
+begin
+  assume hex,
+  cases' hex,
+  cases' h,
+  repeat {rw subst at h_1},
+  rw ite at h_1,
+  cases' h_1,
+  cases' h_1_1
+end
+
+lemma test_name_shadow : 
+  ELet "x" (ELet "x" (EVal (VNat 1)) 
+              (EOp PlusOp (EVar "x") (EVal (VNat 2)))) -- = 3
+    (ELet "x" (EVal (VNat 0)) 
+        (EOp EqOp (EVar "x") (EVal (VNat 0)))) ⟹ VBool true :=
+begin
+  apply RunLet,
+  { apply RunLet,
+    { apply RunVal },
+    { repeat {rw subst},
+      apply RunOp,
+      simp,
+      exact RunVal,
+      exact RunVal } },
+  { repeat {rw subst},
+    simp,
+    apply RunLet,
+    repeat {apply RunVal},
+    repeat {rw subst},
+    simp,
+    have heq : VBool tt = eval 0 0 EqOp := by refl,
+    rw heq,
+    apply RunOp,
+    exact RunVal,
+    exact RunVal
+  }
+end
+
+lemma test_ext : 
+  ([],
+   [IPush (VNat 0),
+    IPush (VNat 1),
+    IOpenScope "x",
+    IOpenScope "y",
+    IPush (VNat 2),
+    ILookup "x",
+    ICloseScope,
+    IOp PlusOp], []) ⟹ᵥₘ [VNat 3] :=
+begin
+  apply RunPush,
+  apply RunPush,
+  apply RunOpenScope,
+  apply RunOpenScope,
+  apply RunPush,
+  apply RunLookup,
+  { apply bound.btail,
+    apply bound.bhead },
+  apply RunCloseScope,
+  have h : VNat 3 = eval 1 2 PlusOp := by refl,
+  rw h,
+  apply RunOpInstr,
+  exact RunEmpty
+end
